coq/PrimitiveProperties.v
@@ -12,11 +12,11 @@ Ltac min_t :=
 
 Lemma slice_end :
   forall sz sz' (v : bits (sz + sz')),
-    slice sz sz' v = vect_skipn_plus sz v.
+    Bits.slice sz sz' v = vect_skipn_plus sz v.
 Proof.
   intros.
   apply vect_to_list_inj.
-  unfold slice, vect_skipn_plus, vect_extend_end_firstn, vect_extend_end.
+  unfold Bits.slice, vect_skipn_plus, vect_extend_end_firstn, vect_extend_end.
   autorewrite with vect_to_list.
   min_t; rewrite Nat.sub_diag by omega; cbn.
   rewrite app_nil_r.
@@ -28,12 +28,12 @@ Qed.
 Lemma slice_front :
   forall n sz (v: bits (n + sz)) offset width,
     offset + width <= n ->
-    slice offset width v =
-    slice offset width (vect_firstn_plus n v).
+    Bits.slice offset width v =
+    Bits.slice offset width (vect_firstn_plus n v).
 Proof.
   intros.
   apply vect_to_list_inj.
-  unfold slice, vect_extend_end_firstn, vect_extend_end, vect_firstn_plus.
+  unfold Bits.slice, vect_extend_end_firstn, vect_extend_end, vect_firstn_plus.
   autorewrite with vect_to_list.
   rewrite skipn_firstn, firstn_firstn.
   min_t; reflexivity.
@@ -65,11 +65,11 @@ Qed.
 
 Lemma slice_subst_end :
   forall sz0 sz (bs0: bits (sz0 + sz)) (bs: bits sz),
-    slice_subst sz0 sz bs0 bs = Bits.app bs (fst (Bits.split bs0)).
+    Bits.slice_subst sz0 sz bs0 bs = Bits.app bs (fst (Bits.split bs0)).
 Proof.
   unfold Bits.split; intros; rewrite vect_split_firstn_skipn; cbn.
   apply vect_to_list_inj.
-  unfold slice_subst, vect_skipn_plus, vect_firstn_plus, vect_extend_end_firstn, vect_extend_end.
+  unfold Bits.slice_subst, vect_skipn_plus, vect_firstn_plus, vect_extend_end_firstn, vect_extend_end.
   autorewrite with vect_to_list.
   rewrite !firstn_app.
   rewrite firstn_length_le by (rewrite vect_to_list_length; omega).
@@ -82,13 +82,13 @@ Qed.
 Lemma slice_subst_front :
   forall sz0 sz width (bs0: bits (sz0 + sz)) (bs: bits width) offset,
     offset + width <= sz0 ->
-    slice_subst offset width bs0 bs =
-    Bits.app (vect_skipn_plus sz0 bs0) (slice_subst offset width (vect_firstn_plus sz0 bs0) bs).
+    Bits.slice_subst offset width bs0 bs =
+    Bits.app (vect_skipn_plus sz0 bs0) (Bits.slice_subst offset width (vect_firstn_plus sz0 bs0) bs).
 Proof.
   clear.
   intros.
   apply vect_to_list_inj;
-    unfold slice_subst, vect_skipn_plus, vect_firstn_plus, vect_extend_end_firstn, vect_extend_end.
+    unfold Bits.slice_subst, vect_skipn_plus, vect_firstn_plus, vect_extend_end_firstn, vect_extend_end.
   autorewrite with vect_to_list.
   rewrite !firstn_app.
   rewrite firstn_length_le by (rewrite vect_to_list_length; omega).
@@ -129,7 +129,7 @@ Proof. _eq_t. Qed.
 
 Lemma get_field_bits_slice:
   forall {sig} (idx : struct_index sig) (a : type_denote (struct_t sig)),
-    slice (field_offset_right sig idx) (field_sz sig idx) (bits_of_value a) =
+    Bits.slice (field_offset_right sig idx) (field_sz sig idx) (bits_of_value a) =
     bits_of_value (get_field (struct_fields sig) a idx).
 Proof.
   intro sig;
@@ -147,7 +147,7 @@ Qed.
 Lemma get_element_bits_slice:
   forall (sig : array_sig) (idx : array_index sig)
     (a : vect (array_type sig) (array_len sig)),
-    slice (element_offset_right sig idx) (element_sz sig)
+    Bits.slice (element_offset_right sig idx) (element_sz sig)
           (Bits.appn (vect_map bits_of_value a)) =
     bits_of_value (vect_nth a idx).
 Proof.
@@ -165,7 +165,7 @@ Qed.
 
 Lemma subst_field_bits_slice_subst:
   forall {sig} (idx : struct_index sig) (a1 : type_denote (struct_t sig)) (a2 : field_type sig idx),
-    slice_subst (field_offset_right sig idx) (field_sz sig idx) (bits_of_value a1) (bits_of_value a2) =
+    Bits.slice_subst (field_offset_right sig idx) (field_sz sig idx) (bits_of_value a1) (bits_of_value a2) =
     bits_of_value (tau := struct_t _) (subst_field (struct_fields sig) a1 idx a2).
 Proof.
   intro sig;
@@ -183,7 +183,7 @@ Qed.
 Lemma subst_element_bits_slice_subst:
   forall (sig : array_sig) (idx : array_index sig)
     (a1 : vect (array_type sig) (array_len sig)) (a2 : array_type sig),
-    slice_subst (element_offset_right sig idx) (element_sz sig)
+    Bits.slice_subst (element_offset_right sig idx) (element_sz sig)
                 (Bits.appn (vect_map bits_of_value a1)) (bits_of_value a2) =
     Bits.appn (vect_map bits_of_value (vect_replace a1 idx a2)).
 Proof.
@@ -215,18 +215,18 @@ Definition slice_subst_impl {sz} offset {width} (a1: bits sz) (a2: bits width) :
   match le_gt_dec offset sz with
   | left pr =>
     rew le_plus_minus_r offset sz pr in
-      ((BitFuns.slice 0 offset a1) ++
+      ((Bits.slice 0 offset a1) ++
        (match le_gt_dec width (sz - offset) with
         | left pr =>
           rew le_plus_minus_r width (sz - offset) pr in
-            (a2 ++ BitFuns.slice (offset + width) (sz - offset - width) a1)
-        | right _ => BitFuns.slice 0 (sz - offset) a2
+            (a2 ++ Bits.slice (offset + width) (sz - offset - width) a1)
+        | right _ => Bits.slice 0 (sz - offset) a2
         end))%vect
   | right _ => a1
   end.
 
-Hint Unfold BitFuns.slice : vect_to_list.
-Hint Unfold BitFuns.slice_subst : vect_to_list.
+Hint Unfold Bits.slice : vect_to_list.
+Hint Unfold Bits.slice_subst : vect_to_list.
 Hint Unfold slice_subst_impl : vect_to_list.
 Hint Unfold vect_extend_end : vect_to_list.
 Hint Unfold vect_extend_end_firstn : vect_to_list.
@@ -245,7 +245,7 @@ Ltac vect_to_list_t :=
 
 Lemma slice_subst_impl_correct :
   forall {sz} offset {width} (a1: bits sz) (a2: bits width),
-    BitFuns.slice_subst offset width a1 a2 =
+    Bits.slice_subst offset width a1 a2 =
     slice_subst_impl offset a1 a2.
 Proof.
   intros; vect_to_list_t.
@@ -259,7 +259,7 @@ Qed.
 
 Lemma slice_full {sz}:
   forall (bs: bits sz),
-    BitFuns.slice 0 sz bs = bs.
+    Bits.slice 0 sz bs = bs.
 Proof.
   intros; vect_to_list_t.
   rewrite (firstn_all2 (n := sz)) by (autorewrite with vect_to_list; omega);
@@ -268,7 +268,7 @@ Qed.
 
 Lemma slice_concat_l {sz1 sz2} :
   forall (bs1: bits sz1) (bs2: bits sz2),
-    BitFuns.slice 0 sz1 (bs1 ++ bs2)%vect = bs1.
+    Bits.slice 0 sz1 (bs1 ++ bs2)%vect = bs1.
 Proof.
   intros; vect_to_list_t.
   rewrite (firstn_all2 (n := sz1)) by (autorewrite with vect_to_list; omega);
@@ -277,7 +277,7 @@ Qed.
 
 Lemma slice_concat_r {sz1 sz2} :
   forall (bs1: bits sz1) (bs2: bits sz2),
-    BitFuns.slice sz1 sz2 (bs1 ++ bs2)%vect = bs2.
+    Bits.slice sz1 sz2 (bs1 ++ bs2)%vect = bs2.
 Proof.
   intros; vect_to_list_t.
   rewrite (skipn_all2 (n := sz1)) by (autorewrite with vect_to_list; omega).
@@ -414,5 +414,4 @@ Section Arithmetic.
     rewrite Bits.to_N_rew, Bits.to_N_app, Bits.to_N_zeroes, N.mul_0_l, N.add_0_l.
     reflexivity.
   Qed.
-
 End Arithmetic.
